01Source/SourceLanguage.thy
@@ -12,87 +12,131 @@ here, since our language as it stands does in fact admit unnormalizable terms li
 lower our sights to the simply-typed subset of our language and be able to prove normalization then.
 As for substitution, for now we take the brute-force approach of renaming every binder to a fresh 
 variable every time we substitute past it. We will shortly switch to a nameless Debruijn-index 
-representation to make substitution simpler, but we want to keep out source language as close to an 
+representation to make substitution simpler, but we want to keep our source language as close to an 
 intuitive, "human-readable" version as possible. After all, changing this sort of behaviour to one 
 more easily implemented on a computer is the essence of compilation.\<close>
 
+text \<open>Our concrete datatype is parameterized on an annotation on each binder; this will enable us to
+reuse the same datatype for the typed version.\<close>
+
 (* TODO: products and sums *)
 
-datatype expr\<^sub>s = 
+datatype 'a expr\<^sub>s = 
   Var\<^sub>s var
   | Const\<^sub>s nat
-  | Lam\<^sub>s var expr\<^sub>s
-  | App\<^sub>s expr\<^sub>s expr\<^sub>s
+  | Lam\<^sub>s var 'a "'a expr\<^sub>s"
+  | App\<^sub>s "'a expr\<^sub>s" "'a expr\<^sub>s"
 
 text \<open>Only numbers and lambda-abstractions are values:\<close>
 
-primrec "value" :: "expr\<^sub>s \<Rightarrow> bool" where
-  "value (Var\<^sub>s x) = False"
-| "value (Const\<^sub>s k) = True" 
-| "value (Lam\<^sub>s x e) = True" 
-| "value (App\<^sub>s e\<^sub>1 e\<^sub>2) = False" 
+primrec value\<^sub>s :: "'a expr\<^sub>s \<Rightarrow> bool" where
+  "value\<^sub>s (Var\<^sub>s x) = False"
+| "value\<^sub>s (Const\<^sub>s n) = True" 
+| "value\<^sub>s (Lam\<^sub>s x t e) = True" 
+| "value\<^sub>s (App\<^sub>s e\<^sub>1 e\<^sub>2) = False" 
+
+text \<open>We define free variables in the usual way:\<close>
+
+primrec free_vars\<^sub>s :: "'a expr\<^sub>s \<Rightarrow> var set" where
+  "free_vars\<^sub>s (Var\<^sub>s x) = {x}"
+| "free_vars\<^sub>s (Const\<^sub>s k) = {}"
+| "free_vars\<^sub>s (Lam\<^sub>s x t e) = free_vars\<^sub>s e - {x}"
+| "free_vars\<^sub>s (App\<^sub>s e\<^sub>1 e\<^sub>2) = free_vars\<^sub>s e\<^sub>1 \<union> free_vars\<^sub>s e\<^sub>2"
 
 text \<open>Our capture-avoiding substitution requires some helper methods. First, a function to gather up 
-all variables in an expression:\<close>
+all variables in an expression, even bound ones:\<close>
 
-primrec all_vars :: "expr\<^sub>s \<Rightarrow> var set" where
-  "all_vars (Var\<^sub>s x) = {x}"
-| "all_vars (Const\<^sub>s k) = {}"
-| "all_vars (Lam\<^sub>s x e) = insert x (all_vars e)"
-| "all_vars (App\<^sub>s e\<^sub>1 e\<^sub>2) = all_vars e\<^sub>1 \<union> all_vars e\<^sub>2"
+primrec all_vars\<^sub>s :: "'a expr\<^sub>s \<Rightarrow> var set" where
+  "all_vars\<^sub>s (Var\<^sub>s x) = {x}"
+| "all_vars\<^sub>s (Const\<^sub>s n) = {}"
+| "all_vars\<^sub>s (Lam\<^sub>s x t e) = insert x (all_vars\<^sub>s e)"
+| "all_vars\<^sub>s (App\<^sub>s e\<^sub>1 e\<^sub>2) = all_vars\<^sub>s e\<^sub>1 \<union> all_vars\<^sub>s e\<^sub>2"
 
-lemma all_vars_finite: "finite (all_vars e)"
+lemma all_vars_finite [simp]: "finite (all_vars\<^sub>s e)"
   by (induction e) simp_all
 
-text \<open>Next, we make a limited form of substitution that simply swaps one variable for another. Note 
-that this function is unsafe if the replacement variable is bound in the expression; we will only 
-ever use it in \<open>subst\<close>, where we generate a fresh variable for it.\<close>
+text \<open>Next, we define a limited form of substitution that simply swaps one variable for another. 
+Note that this function is unsafe if the replacement variable is bound in the expression; we will 
+only ever use it in \<open>subst\<^sub>s\<close>, where we generate a fresh variable for it.\<close>
 
-primrec subst_var :: "var \<Rightarrow> var \<Rightarrow> expr\<^sub>s \<Rightarrow> expr\<^sub>s" where
-  "subst_var x x' (Var\<^sub>s y) = Var\<^sub>s (if x = y then x' else y)"
-| "subst_var x x' (Const\<^sub>s k) = Const\<^sub>s k"
-| "subst_var x x' (Lam\<^sub>s y e) = Lam\<^sub>s y (if x = y then e else subst_var x x' e)"
-| "subst_var x x' (App\<^sub>s e\<^sub>1 e\<^sub>2) = App\<^sub>s (subst_var x x' e\<^sub>1) (subst_var x x' e\<^sub>2)"
+primrec subst_var\<^sub>s :: "var \<Rightarrow> var \<Rightarrow> 'a expr\<^sub>s \<Rightarrow> 'a expr\<^sub>s" where
+  "subst_var\<^sub>s x x' (Var\<^sub>s y) = Var\<^sub>s (if x = y then x' else y)"
+| "subst_var\<^sub>s x x' (Const\<^sub>s n) = Const\<^sub>s n"
+| "subst_var\<^sub>s x x' (Lam\<^sub>s y t e) = Lam\<^sub>s y t (if x = y then e else subst_var\<^sub>s x x' e)"
+| "subst_var\<^sub>s x x' (App\<^sub>s e\<^sub>1 e\<^sub>2) = App\<^sub>s (subst_var\<^sub>s x x' e\<^sub>1) (subst_var\<^sub>s x x' e\<^sub>2)"
 
-lemma size_subst_var [simp]: "size (subst_var x x' e) = size e"
+lemma size_subst_var [simp]: "size (subst_var\<^sub>s x x' e) = size e"
   by (induction e) simp_all
 
 text \<open>Finally, our capture-avoiding substitution function. As noted above, we rename every binder 
 every time we pass one, using the \<open>subst_var\<close> helper method to avoid an infinite regress. Indeed, we 
 still need the \<open>size_subst_var\<close> lemma just to prove termination.\<close> 
 
-fun subst\<^sub>s :: "var \<Rightarrow> expr\<^sub>s \<Rightarrow> expr\<^sub>s \<Rightarrow> expr\<^sub>s" where
+fun subst\<^sub>s :: "var \<Rightarrow> 'a expr\<^sub>s \<Rightarrow> 'a expr\<^sub>s \<Rightarrow> 'a expr\<^sub>s" where
   "subst\<^sub>s x e' (Var\<^sub>s y) = (if x = y then e' else Var\<^sub>s y)"
-| "subst\<^sub>s x e' (Const\<^sub>s k) = Const\<^sub>s k"
-| "subst\<^sub>s x e' (Lam\<^sub>s y e) = (
-    let z = fresh (all_vars e' \<union> all_vars e \<union> {x, y})
-    in Lam\<^sub>s z (subst\<^sub>s x e' (subst_var y z e)))"
+| "subst\<^sub>s x e' (Const\<^sub>s n) = Const\<^sub>s n"
+| "subst\<^sub>s x e' (Lam\<^sub>s y t e) = (
+    let z = fresh (all_vars\<^sub>s e' \<union> all_vars\<^sub>s e \<union> {x, y})
+    in Lam\<^sub>s z t (subst\<^sub>s x e' (subst_var\<^sub>s y z e)))"
 | "subst\<^sub>s x e' (App\<^sub>s e\<^sub>1 e\<^sub>2) = App\<^sub>s (subst\<^sub>s x e' e\<^sub>1) (subst\<^sub>s x e' e\<^sub>2)"
+
+lemma free_vars_subst_var [simp]: "free_vars\<^sub>s e \<subseteq> insert x xs \<Longrightarrow> 
+ free_vars\<^sub>s (subst_var\<^sub>s x x' e) \<subseteq> insert x' xs"
+proof (induction e arbitrary: xs)
+  case (Lam\<^sub>s y t e)
+  hence "free_vars\<^sub>s e \<subseteq> insert x (insert y xs)" by auto
+  with Lam\<^sub>s have "free_vars\<^sub>s (subst_var\<^sub>s x x' e) \<subseteq> insert x' (insert y xs)" by simp
+  with Lam\<^sub>s show ?case by auto
+qed auto
+
+lemma free_vars_subst [simp]: "free_vars\<^sub>s e \<subseteq> insert x xs \<Longrightarrow> free_vars\<^sub>s e' \<subseteq> xs \<Longrightarrow> 
+  free_vars\<^sub>s (subst\<^sub>s x e' e) \<subseteq> xs"
+proof (induction x e' e arbitrary: xs rule: subst\<^sub>s.induct)
+  case (3 x e' y t e)
+  let ?z = "fresh (all_vars\<^sub>s e' \<union> all_vars\<^sub>s e \<union> {x, y})"
+  from 3 have "free_vars\<^sub>s e \<subseteq> insert y (insert x xs)" by auto
+  hence "free_vars\<^sub>s (subst_var\<^sub>s y ?z e) \<subseteq> insert ?z (insert x xs)" by simp
+  hence "free_vars\<^sub>s (subst_var\<^sub>s y ?z e) \<subseteq> insert x (insert ?z xs)" by auto
+  with 3 show ?case by (auto simp add: Let_def)
+qed auto
 
 text \<open>Now, we define big-step applicative-order evaluation. It is represented by an inductive 
 relation rather than an evaluation function because, of course, some source expressions do not have 
 a normal form. However, even once we prove termination for later stages, we will mostly continue to 
 use an inductive definition of evaluation simply because it is easier to write and work with.\<close> 
 
-inductive eval\<^sub>s :: "expr\<^sub>s \<Rightarrow> expr\<^sub>s \<Rightarrow> bool" (infix "\<Down>" 50) where
+inductive eval\<^sub>s :: "'a expr\<^sub>s \<Rightarrow> 'a expr\<^sub>s \<Rightarrow> bool" (infix "\<Down>" 50) where
   ev\<^sub>s_const [simp]: "Const\<^sub>s k \<Down> Const\<^sub>s k"
-| ev\<^sub>s_lam [simp]: "Lam\<^sub>s x e \<Down> Lam\<^sub>s x e"
-| ev\<^sub>s_app [simp]: "e\<^sub>1 \<Down> Lam\<^sub>s x e\<^sub>1' \<Longrightarrow> e\<^sub>2 \<Down> v\<^sub>2 \<Longrightarrow> subst\<^sub>s x v\<^sub>2 e\<^sub>1' \<Down> v \<Longrightarrow> App\<^sub>s e\<^sub>1 e\<^sub>2 \<Down> v"
+| ev\<^sub>s_lam [simp]: "Lam\<^sub>s x t e \<Down> Lam\<^sub>s x t e"
+| ev\<^sub>s_app [simp]: "e\<^sub>1 \<Down> Lam\<^sub>s x t e\<^sub>1' \<Longrightarrow> e\<^sub>2 \<Down> v\<^sub>2 \<Longrightarrow> subst\<^sub>s x v\<^sub>2 e\<^sub>1' \<Down> v \<Longrightarrow> App\<^sub>s e\<^sub>1 e\<^sub>2 \<Down> v"
+
+lemma free_vars_eval [simp]: "e \<Down> v \<Longrightarrow> free_vars\<^sub>s e = {} \<Longrightarrow> free_vars\<^sub>s v = {}"
+proof (induction e v rule: eval\<^sub>s.induct)
+  case (ev\<^sub>s_app e\<^sub>1 x t e\<^sub>1' e\<^sub>2 v\<^sub>2 v)
+  hence "free_vars\<^sub>s e\<^sub>1' \<subseteq> insert x {} \<and> free_vars\<^sub>s v\<^sub>2 \<subseteq> {}" by simp
+  hence "free_vars\<^sub>s (subst\<^sub>s x v\<^sub>2 e\<^sub>1') \<subseteq> {}" by (metis free_vars_subst)
+  with ev\<^sub>s_app show ?case by simp
+qed simp_all
+
+lemma eval_to_value [simp]: "e \<Down> v \<Longrightarrow> value\<^sub>s v"
+  by (induction e v rule: eval\<^sub>s.induct) simp_all
+
+lemma val_no_eval: "e \<Down> v \<Longrightarrow> value\<^sub>s e \<Longrightarrow> v = e"
+  by (induction e v rule: eval\<^sub>s.induct) simp_all
 
 text \<open>Since our language is untyped, we cannot prove (or even express) the progress and preservation 
 theorems. However, we can prove determinism of evaluation:\<close>
 
-theorem determinismn: "e \<Down> v \<Longrightarrow> e \<Down> v' \<Longrightarrow> v = v'"
+theorem determinism\<^sub>s: "e \<Down> v \<Longrightarrow> e \<Down> v' \<Longrightarrow> v = v'"
 proof (induction e v arbitrary: v' rule: eval\<^sub>s.induct)
   case (ev\<^sub>s_const k)
-  thus ?case by (induction "Const\<^sub>s k" v' rule: eval\<^sub>s.induct) simp_all
+  thus ?case by (induction rule: eval\<^sub>s.cases) simp_all
 next
   case (ev\<^sub>s_lam x e)
-  thus ?case by (induction "Lam\<^sub>s x e" v' rule: eval\<^sub>s.induct) simp_all
+  thus ?case by (induction rule: eval\<^sub>s.cases) simp_all
 next
   case (ev\<^sub>s_app e\<^sub>1 x e\<^sub>1' e\<^sub>2 v\<^sub>2 v)
-  from ev\<^sub>s_app(7, 1, 2, 3, 4, 5, 6) show ?case 
-    by (induction "App\<^sub>s e\<^sub>1 e\<^sub>2" v' rule: eval\<^sub>s.induct) blast+
+  from ev\<^sub>s_app(7, 1, 2, 3, 4, 5, 6) show ?case by (induction rule: eval\<^sub>s.cases) blast+
 qed
 
 end
