03Debruijn/NameRemoval.thy
@@ -2,14 +2,14 @@ theory NameRemoval
   imports "../02Typed/Typechecking" BigStep "../00Utils/AssocList"
 begin
 
-fun convert' :: "var list \<Rightarrow> texpr \<Rightarrow> dexpr" where
-  "convert' \<Phi> (TVar x) = DVar (the (idx_of \<Phi> x))"
-| "convert' \<Phi> (TConst k) = DConst k"
-| "convert' \<Phi> (TLam x t e) = DLam t (convert' (insert_at 0 x \<Phi>) e)"
-| "convert' \<Phi> (TApp e\<^sub>1 e\<^sub>2) = DApp (convert' \<Phi> e\<^sub>1) (convert' \<Phi> e\<^sub>2)"
+fun convert' :: "var list \<Rightarrow> ty expr\<^sub>s \<Rightarrow> dexpr" where
+  "convert' \<Phi> (Var\<^sub>s x) = DVar (the (idx_of \<Phi> x))"
+| "convert' \<Phi> (Const\<^sub>s k) = DConst k"
+| "convert' \<Phi> (Lam\<^sub>s x t e) = DLam t (convert' (insert_at 0 x \<Phi>) e)"
+| "convert' \<Phi> (App\<^sub>s e\<^sub>1 e\<^sub>2) = DApp (convert' \<Phi> e\<^sub>1) (convert' \<Phi> e\<^sub>2)"
 
-definition convert :: "texpr \<Rightarrow> dexpr" where
-  "convert e = convert' [] e"
+definition convert :: "ty expr\<^sub>s \<Rightarrow> dexpr" where
+  "convert e \<equiv> convert' [] e"
 
 lemma [simp]: "map_of \<Gamma> \<turnstile>\<^sub>n e : t \<Longrightarrow> mset (map fst \<Gamma>) = mset \<Phi> \<Longrightarrow> 
   map_by_assoc_list \<Gamma> \<Phi> \<turnstile>\<^sub>d convert' \<Phi> e : t"
@@ -34,22 +34,22 @@ proof (unfold convert_def)
   thus "[] \<turnstile>\<^sub>d convert' [] e : t" by (simp add: \<Gamma>_def \<Phi>_def)
 qed
 
-lemma [simp]: "valt e \<Longrightarrow> vald (convert' \<Phi> e)"
+lemma [simp]: "value\<^sub>s e \<Longrightarrow> vald (convert' \<Phi> e)"
   by (induction e) (simp_all add: Let_def)
 
-lemma [simp]: "y \<notin> all_varst e \<Longrightarrow> x \<le> length \<Phi> \<Longrightarrow> free_varst e \<subseteq> set \<Phi> \<Longrightarrow>
+lemma [simp]: "y \<notin> all_vars\<^sub>s e \<Longrightarrow> x \<le> length \<Phi> \<Longrightarrow> free_vars\<^sub>s e \<subseteq> set \<Phi> \<Longrightarrow>
   convert' (insert_at x y \<Phi>) e = incrd x (convert' \<Phi> e)"
 proof (induction e arbitrary: x \<Phi>)
-  case (TVar z)
+  case (Var\<^sub>s z)
   moreover then obtain w where "idx_of \<Phi> z = Some w" by fastforce
   ultimately show ?case by simp
 next
-  case (TLam z t e)
-  moreover hence "free_varst e \<subseteq> set (insert_at 0 z \<Phi>)" by auto
+  case (Lam\<^sub>s z t e)
+  moreover hence "free_vars\<^sub>s e \<subseteq> set (insert_at 0 z \<Phi>)" by auto
   ultimately show ?case by simp
 qed simp_all
 
-lemma [simp]: "x' \<notin> all_varst e \<Longrightarrow> a \<le> length \<Phi> \<Longrightarrow> idx_of \<Phi> x = Some y \<Longrightarrow> a > y \<Longrightarrow> 
+lemma [simp]: "x' \<notin> all_vars\<^sub>s e \<Longrightarrow> a \<le> length \<Phi> \<Longrightarrow> idx_of \<Phi> x = Some y \<Longrightarrow> a > y \<Longrightarrow> 
     convert' (insert_at a x \<Phi>) e = convert' (insert_at a x' \<Phi>) e"
   by (induction e arbitrary: a \<Phi> y) (auto simp add: incr_min split: option.splits)
 
@@ -59,25 +59,25 @@ abbreviation precede :: "nat \<Rightarrow> 'a \<Rightarrow> 'a list \<Rightarrow
 lemma [simp]: "0 precedes a in as"
   by (simp split: option.splits)
 
-lemma [simp]: "y \<le> length \<Phi> \<Longrightarrow> y precedes x in \<Phi> \<Longrightarrow> y precedes x' in \<Phi> \<Longrightarrow> x' \<notin> all_varst e \<Longrightarrow> 
-  free_varst e \<subseteq> insert x (set \<Phi>) \<Longrightarrow> 
-    convert' (insert_at y x' \<Phi>) (subst_vart x x' e) = convert' (insert_at y x \<Phi>) e"
+lemma [simp]: "y \<le> length \<Phi> \<Longrightarrow> y precedes x in \<Phi> \<Longrightarrow> y precedes x' in \<Phi> \<Longrightarrow> x' \<notin> all_vars\<^sub>s e \<Longrightarrow> 
+  free_vars\<^sub>s e \<subseteq> insert x (set \<Phi>) \<Longrightarrow> 
+    convert' (insert_at y x' \<Phi>) (subst_var\<^sub>s x x' e) = convert' (insert_at y x \<Phi>) e"
 proof (induction e arbitrary: y \<Phi>)
-  case (TLam z t e)
+  case (Lam\<^sub>s z t e)
   thus ?case
   proof (cases "x = z")
     case False
-    with TLam have X: "Suc y precedes x in insert_at 0 z \<Phi>" by (simp split: option.splits) 
-    from TLam have Y: "Suc y precedes x' in insert_at 0 z \<Phi>" by (simp split: option.splits) 
-    from TLam have "free_varst e \<subseteq> insert x (set (insert_at 0 z \<Phi>))" by auto
-    with TLam False X Y show ?thesis by simp
+    with Lam\<^sub>s have X: "Suc y precedes x in insert_at 0 z \<Phi>" by (simp split: option.splits) 
+    from Lam\<^sub>s have Y: "Suc y precedes x' in insert_at 0 z \<Phi>" by (simp split: option.splits) 
+    from Lam\<^sub>s have "free_vars\<^sub>s e \<subseteq> insert x (set (insert_at 0 z \<Phi>))" by auto
+    with Lam\<^sub>s False X Y show ?thesis by simp
   qed (simp_all split: option.splits)
 qed (auto split: option.splits)
 
-lemma convert_subst [simp]: "y \<le> length \<Phi> \<Longrightarrow> x \<notin> set \<Phi> \<Longrightarrow> free_varst e \<subseteq> insert x (set \<Phi>) \<Longrightarrow>
-  free_varst e' \<subseteq> set \<Phi> \<Longrightarrow>
-    convert' \<Phi> (substt x e' e) = substd y (convert' \<Phi> e') (convert' (insert_at y x \<Phi>) e)" 
-proof (induction x e' e arbitrary: \<Phi> y rule: substt.induct)
+lemma convert_subst [simp]: "y \<le> length \<Phi> \<Longrightarrow> x \<notin> set \<Phi> \<Longrightarrow> free_vars\<^sub>s e \<subseteq> insert x (set \<Phi>) \<Longrightarrow>
+  free_vars\<^sub>s e' \<subseteq> set \<Phi> \<Longrightarrow>
+    convert' \<Phi> (subst\<^sub>s x e' e) = substd y (convert' \<Phi> e') (convert' (insert_at y x \<Phi>) e)" 
+proof (induction x e' e arbitrary: \<Phi> y rule: subst\<^sub>s.induct)
   case (1 x e' z)
   thus ?case
   proof (cases "idx_of \<Phi> z")
@@ -87,96 +87,96 @@ proof (induction x e' e arbitrary: \<Phi> y rule: substt.induct)
   qed simp_all
 next
   case (3 x e' z t e)
-  let ?z' = "fresh (all_varst e' \<union> all_varst e \<union> {x, z})"
-  have "finite (all_varst e' \<union> all_varst e \<union> {x, z})" by simp
-  hence Z: "?z' \<notin> all_varst e' \<union> all_varst e \<union> {x, z}" by (metis fresh_is_fresh)
-  from 3 Z have X: "free_varst e' \<subseteq> set (insert_at 0 ?z' \<Phi>)" by auto
-  from 3 have "free_varst e \<subseteq> insert z (insert x (set \<Phi>))" by auto
-  with Z have "free_varst (subst_vart z ?z' e) \<subseteq> insert ?z' (insert x (set \<Phi>))" by auto
-  hence "free_varst (subst_vart z ?z' e) \<subseteq> insert x (set (insert_at 0 ?z' \<Phi>))" by auto
-  with 3 X Z have H: "convert' (insert_at 0 ?z' \<Phi>) (substt x e' (subst_vart z ?z' e)) = 
+  let ?z' = "fresh (all_vars\<^sub>s e' \<union> all_vars\<^sub>s e \<union> {x, z})"
+  have "finite (all_vars\<^sub>s e' \<union> all_vars\<^sub>s e \<union> {x, z})" by simp
+  hence Z: "?z' \<notin> all_vars\<^sub>s e' \<union> all_vars\<^sub>s e \<union> {x, z}" by (metis fresh_is_fresh)
+  from 3 Z have X: "free_vars\<^sub>s e' \<subseteq> set (insert_at 0 ?z' \<Phi>)" by auto
+  from 3 have "free_vars\<^sub>s e \<subseteq> insert z (insert x (set \<Phi>))" by auto
+  with Z have "free_vars\<^sub>s (subst_var\<^sub>s z ?z' e) \<subseteq> insert ?z' (insert x (set \<Phi>))" by auto
+  hence "free_vars\<^sub>s (subst_var\<^sub>s z ?z' e) \<subseteq> insert x (set (insert_at 0 ?z' \<Phi>))" by auto
+  with 3 X Z have H: "convert' (insert_at 0 ?z' \<Phi>) (subst\<^sub>s x e' (subst_var\<^sub>s z ?z' e)) = 
     substd (Suc y) (convert' (insert_at 0 ?z' \<Phi>) e') 
-      (convert' (insert_at (Suc y) x (insert_at 0 ?z' \<Phi>)) (subst_vart z ?z' e))" by fastforce
-  from 3 have "free_varst e \<subseteq> insert z (set (insert_at y x \<Phi>))" by auto
-  with Z have "convert' (insert_at 0 ?z' (insert_at y x \<Phi>)) (subst_vart z ?z' e) =
+      (convert' (insert_at (Suc y) x (insert_at 0 ?z' \<Phi>)) (subst_var\<^sub>s z ?z' e))" by fastforce
+  from 3 have "free_vars\<^sub>s e \<subseteq> insert z (set (insert_at y x \<Phi>))" by auto
+  with Z have "convert' (insert_at 0 ?z' (insert_at y x \<Phi>)) (subst_var\<^sub>s z ?z' e) =
     convert' (insert_at 0 z (insert_at y x \<Phi>)) e" by simp
   with 3 Z H show ?case by (simp add: Let_def)
 qed simp_all
 
-theorem correctnd [simp]: "e \<Down>\<^sub>t v \<Longrightarrow> free_varst e = {} \<Longrightarrow> convert e \<Down>\<^sub>d convert v"
-proof (induction e v rule: evalt.induct)
-  case (evt_app e\<^sub>1 x t e\<^sub>1' e\<^sub>2 v\<^sub>2 v)
-  hence "e\<^sub>1 \<Down>\<^sub>t TLam x t e\<^sub>1'" by simp
-  moreover from evt_app have "free_varst e\<^sub>1 = {}" by simp
-  ultimately have "free_varst (TLam x t e\<^sub>1') = {}" by (metis free_vars_evalt)
-  hence X: "free_varst e\<^sub>1' \<subseteq> insert x (set [])" by simp
-  moreover from evt_app have Y: "free_varst v\<^sub>2 \<subseteq> set []" by simp
-  ultimately have "free_varst (substt x v\<^sub>2 e\<^sub>1') \<subseteq> set []" by (metis free_vars_substt)
-  with evt_app X Y show ?case by (simp add: convert_def)
+theorem correctnd [simp]: "e \<Down> v \<Longrightarrow> free_vars\<^sub>s e = {} \<Longrightarrow> convert e \<Down>\<^sub>d convert v"
+proof (induction e v rule: eval\<^sub>s.induct)
+  case (ev\<^sub>s_app e\<^sub>1 x t e\<^sub>1' e\<^sub>2 v\<^sub>2 v)
+  hence "e\<^sub>1 \<Down> Lam\<^sub>s x t e\<^sub>1'" by simp
+  moreover from ev\<^sub>s_app have "free_vars\<^sub>s e\<^sub>1 = {}" by simp
+  ultimately have "free_vars\<^sub>s (Lam\<^sub>s x t e\<^sub>1') = {}" by (metis free_vars_eval)
+  hence X: "free_vars\<^sub>s e\<^sub>1' \<subseteq> insert x (set [])" by simp
+  moreover from ev\<^sub>s_app have Y: "free_vars\<^sub>s v\<^sub>2 \<subseteq> set []" by simp
+  ultimately have "free_vars\<^sub>s (subst\<^sub>s x v\<^sub>2 e\<^sub>1') \<subseteq> set []" by (metis free_vars_subst)
+  with ev\<^sub>s_app X Y show ?case by (simp add: convert_def)
 qed (simp_all add: convert_def)
 
-lemma [simp]: "vald (convert' \<Phi> e) \<Longrightarrow> valt e"
+lemma [simp]: "vald (convert' \<Phi> e) \<Longrightarrow> value\<^sub>s e"
   by (induction e) (simp_all add: Let_def)
 
-lemma convert_val_back: "vald (convert e) \<Longrightarrow> valt e"
+lemma convert_val_back: "vald (convert e) \<Longrightarrow> value\<^sub>s e"
   by (simp add: convert_def)
 
 lemma [dest]: "DApp e\<^sub>d\<^sub>1 e\<^sub>d\<^sub>2 = convert e\<^sub>n \<Longrightarrow> 
-    \<exists>e\<^sub>n\<^sub>1 e\<^sub>n\<^sub>2. e\<^sub>n = TApp e\<^sub>n\<^sub>1 e\<^sub>n\<^sub>2 \<and> e\<^sub>d\<^sub>1 = convert e\<^sub>n\<^sub>1 \<and> e\<^sub>d\<^sub>2 = convert e\<^sub>n\<^sub>2"
+    \<exists>e\<^sub>n\<^sub>1 e\<^sub>n\<^sub>2. e\<^sub>n = App\<^sub>s e\<^sub>n\<^sub>1 e\<^sub>n\<^sub>2 \<and> e\<^sub>d\<^sub>1 = convert e\<^sub>n\<^sub>1 \<and> e\<^sub>d\<^sub>2 = convert e\<^sub>n\<^sub>2"
   by (cases e\<^sub>n) (simp_all add: convert_def)
 
 lemma [dest]: "DLam t e\<^sub>d = convert e\<^sub>n \<Longrightarrow> 
-    \<exists>x e\<^sub>n'. e\<^sub>n = TLam x t e\<^sub>n' \<and> e\<^sub>d = convert' [x] e\<^sub>n'"
+    \<exists>x e\<^sub>n'. e\<^sub>n = Lam\<^sub>s x t e\<^sub>n' \<and> e\<^sub>d = convert' [x] e\<^sub>n'"
   by (cases e\<^sub>n) (simp_all add: convert_def)
 
-theorem completend [simp]: "convert e\<^sub>n \<Down>\<^sub>d v\<^sub>d \<Longrightarrow> free_varst e\<^sub>n = {} \<Longrightarrow> 
-  \<exists>v\<^sub>n. e\<^sub>n \<Down>\<^sub>t v\<^sub>n \<and> v\<^sub>d = convert v\<^sub>n"
+theorem completend [simp]: "convert e\<^sub>n \<Down>\<^sub>d v\<^sub>d \<Longrightarrow> free_vars\<^sub>s e\<^sub>n = {} \<Longrightarrow> 
+  \<exists>v\<^sub>n. e\<^sub>n \<Down> v\<^sub>n \<and> v\<^sub>d = convert v\<^sub>n"
 proof (induction "convert e\<^sub>n" v\<^sub>d arbitrary: e\<^sub>n rule: big_evald.induct)
   case (bevd_const k)
-  hence "e\<^sub>n \<Down>\<^sub>t TConst k \<and> DConst k = convert (TConst k)" by (cases e\<^sub>n) (simp_all add: convert_def)
+  hence "e\<^sub>n \<Down> Const\<^sub>s k \<and> DConst k = convert (Const\<^sub>s k)" by (cases e\<^sub>n) (simp_all add: convert_def)
   thus ?case by fastforce
 next
   case (bevd_lam t e)
-  then obtain x e' where "e\<^sub>n = TLam x t e' \<and> e = convert' [x] e'" 
+  then obtain x e' where "e\<^sub>n = Lam\<^sub>s x t e' \<and> e = convert' [x] e'" 
     by (cases e\<^sub>n) (simp_all add: convert_def)
-  hence "e\<^sub>n \<Down>\<^sub>t TLam x t e' \<and> DLam t e = convert (TLam x t e')" by (simp add: convert_def)
+  hence "e\<^sub>n \<Down> Lam\<^sub>s x t e' \<and> DLam t e = convert (Lam\<^sub>s x t e')" by (simp add: convert_def)
   thus ?case by fastforce
 next
   case (bevd_app e\<^sub>1 t e\<^sub>1' e\<^sub>2 v\<^sub>2 v)
-  then obtain e\<^sub>n\<^sub>1 e\<^sub>n\<^sub>2 where E: "e\<^sub>n = TApp e\<^sub>n\<^sub>1 e\<^sub>n\<^sub>2 \<and> e\<^sub>1 = convert e\<^sub>n\<^sub>1 \<and> e\<^sub>2 = convert e\<^sub>n\<^sub>2" 
+  then obtain e\<^sub>n\<^sub>1 e\<^sub>n\<^sub>2 where E: "e\<^sub>n = App\<^sub>s e\<^sub>n\<^sub>1 e\<^sub>n\<^sub>2 \<and> e\<^sub>1 = convert e\<^sub>n\<^sub>1 \<and> e\<^sub>2 = convert e\<^sub>n\<^sub>2" 
     by (cases e\<^sub>n) (simp_all add: convert_def)
-  with bevd_app obtain v\<^sub>n\<^sub>1 where V1: "e\<^sub>n\<^sub>1 \<Down>\<^sub>t v\<^sub>n\<^sub>1 \<and> DLam t e\<^sub>1' = convert v\<^sub>n\<^sub>1" by fastforce
-  then obtain x e\<^sub>n\<^sub>1' where X: "v\<^sub>n\<^sub>1 = TLam x t e\<^sub>n\<^sub>1' \<and> e\<^sub>1' = convert' [x] e\<^sub>n\<^sub>1'"
+  with bevd_app obtain v\<^sub>n\<^sub>1 where V1: "e\<^sub>n\<^sub>1 \<Down> v\<^sub>n\<^sub>1 \<and> DLam t e\<^sub>1' = convert v\<^sub>n\<^sub>1" by fastforce
+  then obtain x e\<^sub>n\<^sub>1' where X: "v\<^sub>n\<^sub>1 = Lam\<^sub>s x t e\<^sub>n\<^sub>1' \<and> e\<^sub>1' = convert' [x] e\<^sub>n\<^sub>1'"
     by (cases v\<^sub>n\<^sub>1) (simp_all add: convert_def)
-  from bevd_app E obtain v\<^sub>n\<^sub>2 where V2: "e\<^sub>n\<^sub>2 \<Down>\<^sub>t v\<^sub>n\<^sub>2 \<and> v\<^sub>2 = convert v\<^sub>n\<^sub>2" by fastforce
-  from bevd_app E have "free_varst e\<^sub>n\<^sub>1 = {}" by simp
-  with V1 X have "free_varst (TLam x t e\<^sub>n\<^sub>1') = {}" by (metis free_vars_evalt)
-  hence Y: "free_varst e\<^sub>n\<^sub>1' \<subseteq> {x}" by simp
-  from bevd_app E have "free_varst e\<^sub>n\<^sub>2 = {}" by simp
-  with V2 have Z: "free_varst v\<^sub>n\<^sub>2 = {}" by auto
-  with Y have "free_varst (substt x v\<^sub>n\<^sub>2 e\<^sub>n\<^sub>1') = {}" by (metis free_vars_substt subset_empty)
-  with bevd_app X V2 Y Z have "\<exists>v\<^sub>n. substt x v\<^sub>n\<^sub>2 e\<^sub>n\<^sub>1' \<Down>\<^sub>t v\<^sub>n \<and> v = convert v\<^sub>n" 
+  from bevd_app E obtain v\<^sub>n\<^sub>2 where V2: "e\<^sub>n\<^sub>2 \<Down> v\<^sub>n\<^sub>2 \<and> v\<^sub>2 = convert v\<^sub>n\<^sub>2" by fastforce
+  from bevd_app E have "free_vars\<^sub>s e\<^sub>n\<^sub>1 = {}" by simp
+  with V1 X have "free_vars\<^sub>s (Lam\<^sub>s x t e\<^sub>n\<^sub>1') = {}" by (metis free_vars_eval)
+  hence Y: "free_vars\<^sub>s e\<^sub>n\<^sub>1' \<subseteq> {x}" by simp
+  from bevd_app E have "free_vars\<^sub>s e\<^sub>n\<^sub>2 = {}" by simp
+  with V2 have Z: "free_vars\<^sub>s v\<^sub>n\<^sub>2 = {}" by auto
+  with Y have "free_vars\<^sub>s (subst\<^sub>s x v\<^sub>n\<^sub>2 e\<^sub>n\<^sub>1') = {}" by (metis free_vars_subst subset_empty)
+  with bevd_app X V2 Y Z have "\<exists>v\<^sub>n. subst\<^sub>s x v\<^sub>n\<^sub>2 e\<^sub>n\<^sub>1' \<Down> v\<^sub>n \<and> v = convert v\<^sub>n" 
     by (simp add: convert_def)
-  then obtain v\<^sub>n where "substt x v\<^sub>n\<^sub>2 e\<^sub>n\<^sub>1' \<Down>\<^sub>t v\<^sub>n \<and> v = convert v\<^sub>n" by fastforce
-  with V1 X V2 have "TApp e\<^sub>n\<^sub>1 e\<^sub>n\<^sub>2 \<Down>\<^sub>t v\<^sub>n \<and> v = convert v\<^sub>n" by fastforce
+  then obtain v\<^sub>n where "subst\<^sub>s x v\<^sub>n\<^sub>2 e\<^sub>n\<^sub>1' \<Down> v\<^sub>n \<and> v = convert v\<^sub>n" by fastforce
+  with V1 X V2 have "App\<^sub>s e\<^sub>n\<^sub>1 e\<^sub>n\<^sub>2 \<Down> v\<^sub>n \<and> v = convert v\<^sub>n" by fastforce
   with E show ?case by fastforce
 qed
 
 (* Now we can finish the deferred progress lemmas from 01Source/Named and 02Typed/Typed *)
 
-theorem progresst [simp]: "Map.empty \<turnstile>\<^sub>n e : t \<Longrightarrow> \<exists>v. e \<Down>\<^sub>t v"
+theorem progresst [simp]: "Map.empty \<turnstile>\<^sub>n e : t \<Longrightarrow> \<exists>v. e \<Down> v"
 proof -
   assume X: "Map.empty \<turnstile>\<^sub>n e : t"
   hence "[] \<turnstile>\<^sub>d convert e : t" by simp
   then obtain v\<^sub>d where "vald v\<^sub>d \<and> convert e \<Down>\<^sub>d v\<^sub>d" by fastforce
-  with X obtain v\<^sub>n where "e \<Down>\<^sub>t v\<^sub>n \<and> v\<^sub>d = convert v\<^sub>n" by fastforce
+  with X obtain v\<^sub>n where "e \<Down> v\<^sub>n \<and> v\<^sub>d = convert v\<^sub>n" by fastforce
   thus ?thesis by fastforce
 qed
 
 theorem progressn [simp]: "Map.empty \<turnstile>\<^sub>n e : t \<Longrightarrow> \<exists>v. erase e \<Down> v"
 proof -
   assume X: "Map.empty \<turnstile>\<^sub>n e : t"
-  then obtain v\<^sub>t where "e \<Down>\<^sub>t v\<^sub>t" by fastforce
+  then obtain v\<^sub>t where "e \<Down> v\<^sub>t" by fastforce
   hence "erase e \<Down> erase v\<^sub>t" by simp
   thus ?thesis by fastforce
 qed
