02Typed/TypedLanguage.thy
@@ -1,0 +1,92 @@
+theory TypedLanguage
+  imports Type "../01Source/SourceLanguage"
+begin
+
+subsection \<open>Typed Language\<close>
+
+text \<open>Our typed language is almost identical to the untyped source, except there is now a 
+type-annotation on every lambda-abstraction. This small change, of course, produces a great 
+difference in properties, and will take quite a lot of work to establish in the typechecking pass.\<close>
+
+primrec tvarst :: "ty expr\<^sub>s \<Rightarrow> var set" where
+  "tvarst (Var\<^sub>s x) = {}"
+| "tvarst (Const\<^sub>s k) = {}"
+| "tvarst (Lam\<^sub>s x t e) = tvars t \<union> tvarst e"
+| "tvarst (App\<^sub>s e\<^sub>1 e\<^sub>2) = tvarst e\<^sub>1 \<union> tvarst e\<^sub>2"
+
+inductive typecheckn :: "(var \<rightharpoonup> ty) \<Rightarrow> ty expr\<^sub>s \<Rightarrow> ty \<Rightarrow> bool" (infix "\<turnstile>\<^sub>n _ :" 50) where
+  tcn_var [simp]: "\<Gamma> x = Some t \<Longrightarrow> \<Gamma> \<turnstile>\<^sub>n Var\<^sub>s x : t"
+| tcn_const [simp]: "\<Gamma> \<turnstile>\<^sub>n Const\<^sub>s k : Num"
+| tcn_lam [simp]: "\<Gamma>(x \<mapsto> t\<^sub>1) \<turnstile>\<^sub>n e : t\<^sub>2 \<Longrightarrow> \<Gamma> \<turnstile>\<^sub>n Lam\<^sub>s x t\<^sub>1 e : Arrow t\<^sub>1 t\<^sub>2"
+| tcn_app [simp]: "\<Gamma> \<turnstile>\<^sub>n e\<^sub>1 : Arrow t\<^sub>1 t\<^sub>2 \<Longrightarrow> \<Gamma> \<turnstile>\<^sub>n e\<^sub>2 : t\<^sub>1 \<Longrightarrow> \<Gamma> \<turnstile>\<^sub>n App\<^sub>s e\<^sub>1 e\<^sub>2 : t\<^sub>2"
+
+inductive_cases [elim]: "\<Gamma> \<turnstile>\<^sub>n Var\<^sub>s x : t"
+inductive_cases [elim]: "\<Gamma> \<turnstile>\<^sub>n Const\<^sub>s k : t"
+inductive_cases [elim]: "\<Gamma> \<turnstile>\<^sub>n Lam\<^sub>s x t' e : t"
+inductive_cases [elim]: "\<Gamma> \<turnstile>\<^sub>n App\<^sub>s e\<^sub>1 e\<^sub>2 : t"
+
+lemma free_vars_tc [simp]: "\<Gamma> \<turnstile>\<^sub>n e : t \<Longrightarrow> free_vars\<^sub>s e \<subseteq> dom \<Gamma>" 
+  by (induction \<Gamma> e t rule: typecheckn.induct) auto
+
+lemma [simp]: "Map.empty \<turnstile>\<^sub>n e : t \<Longrightarrow> free_vars\<^sub>s e = {}"
+  using free_vars_tc by fastforce
+
+lemma [simp]: "\<Gamma> \<turnstile>\<^sub>n e : t \<Longrightarrow> v \<notin> \<Union> (tvars ` ran \<Gamma>) \<Longrightarrow> v \<notin> tvarst e \<Longrightarrow> v \<notin> tvars t"
+proof (induction \<Gamma> e t rule: typecheckn.induct)
+  case (tcn_lam \<Gamma> x t\<^sub>1 e t\<^sub>2)
+  hence "v \<notin> \<Union> (tvars ` ran (\<Gamma>(x \<mapsto> t\<^sub>1)))" by (auto simp add: ran_def)
+  with tcn_lam show ?case by fastforce
+qed (auto simp add: ran_def)
+
+lemma tcn_tvars [simp]: "\<Gamma> \<turnstile>\<^sub>n e : t \<Longrightarrow> tvars t \<subseteq> tvarst e \<union> \<Union> (tvars ` ran \<Gamma>)"
+proof (induction \<Gamma> e t rule: typecheckn.induct)
+  case (tcn_lam \<Gamma> x t\<^sub>1 e t\<^sub>2)
+  moreover have "\<Union> (tvars ` ran (\<Gamma>(x \<mapsto> t\<^sub>1))) \<subseteq> tvars t\<^sub>1 \<union> \<Union> (tvars ` ran \<Gamma>)" 
+    by (auto simp add: ran_def)
+  ultimately show ?case by (auto simp add: ran_def)
+qed (auto simp add: ran_def)
+
+lemma canonical_base\<^sub>s [dest]: "\<Gamma> \<turnstile>\<^sub>n e : Num \<Longrightarrow> value\<^sub>s e \<Longrightarrow> \<exists>k. e = Const\<^sub>s k"
+  by (induction \<Gamma> e Num rule: typecheckn.induct) simp_all
+
+lemma canonical_arrow\<^sub>s [dest]: "\<Gamma> \<turnstile>\<^sub>n e : Arrow t\<^sub>1 t\<^sub>2 \<Longrightarrow> value\<^sub>s e \<Longrightarrow> 
+    \<exists>x e'. e = Lam\<^sub>s x t\<^sub>1 e' \<and> \<Gamma>(x \<mapsto> t\<^sub>1) \<turnstile>\<^sub>n e' : t\<^sub>2"
+  by (induction \<Gamma> e "Arrow t\<^sub>1 t\<^sub>2" rule: typecheckn.induct) simp_all
+
+(* Progress not directly provable here, due to lack of proof of termination.
+   We prove it in 02Debruijn/NameRemoval *)
+
+lemma [simp]: "\<Gamma> \<turnstile>\<^sub>n e : t \<Longrightarrow> x \<notin> all_vars\<^sub>s e \<Longrightarrow> \<Gamma>(x \<mapsto> t') \<turnstile>\<^sub>n e : t"
+  by (induction \<Gamma> e t rule: typecheckn.induct) (simp_all add: fun_upd_twist)
+
+lemma [simp]: "\<Gamma>(x \<mapsto> t') \<turnstile>\<^sub>n e : t \<Longrightarrow> x' \<notin> all_vars\<^sub>s e \<Longrightarrow> \<Gamma>(x' \<mapsto> t') \<turnstile>\<^sub>n subst_var\<^sub>s x x' e : t"
+proof (induction "\<Gamma>(x \<mapsto> t')" e t arbitrary: \<Gamma> rule: typecheckn.induct)
+  case (tcn_lam y t\<^sub>1 e t\<^sub>2)
+  thus ?case
+  proof (cases "x = y")
+    case False
+    moreover with tcn_lam have "\<Gamma>(y \<mapsto> t\<^sub>1, x' \<mapsto> t') \<turnstile>\<^sub>n subst_var\<^sub>s x x' e : t\<^sub>2" 
+      by (simp add: fun_upd_twist)
+    moreover from tcn_lam have "x' \<noteq> y" by simp
+    ultimately show ?thesis by (simp add: fun_upd_twist)
+  qed (simp_all add: fun_upd_twist)
+qed fastforce+
+
+lemma [simp]: "\<Gamma>(x \<mapsto> t') \<turnstile>\<^sub>n e : t \<Longrightarrow> \<Gamma> \<turnstile>\<^sub>n e' : t' \<Longrightarrow> \<Gamma> \<turnstile>\<^sub>n subst\<^sub>s x e' e : t"
+proof (induction x e' e arbitrary: \<Gamma> t rule: subst\<^sub>s.induct)
+  case (3 x e' y t\<^sub>1 e)
+  then obtain t\<^sub>2 where T: "t = Arrow t\<^sub>1 t\<^sub>2 \<and> \<Gamma>(x \<mapsto> t', y \<mapsto> t\<^sub>1) \<turnstile>\<^sub>n e : t\<^sub>2" by blast
+  let ?z = "fresh (all_vars\<^sub>s e' \<union> all_vars\<^sub>s e \<union> {x, y})"
+  have "finite (all_vars\<^sub>s e' \<union> all_vars\<^sub>s e \<union> {x, y})" by simp
+  hence Z: "?z \<notin> all_vars\<^sub>s e' \<union> all_vars\<^sub>s e \<union> {x, y}" by (metis fresh_is_fresh)
+  with T have "\<Gamma>(x \<mapsto> t', ?z \<mapsto> t\<^sub>1) \<turnstile>\<^sub>n subst_var\<^sub>s y ?z e : t\<^sub>2" by simp
+  with Z have X: "\<Gamma>(?z \<mapsto> t\<^sub>1, x \<mapsto> t') \<turnstile>\<^sub>n subst_var\<^sub>s y ?z e : t\<^sub>2" by (simp add: fun_upd_twist)
+  from 3 Z have "\<Gamma>(?z \<mapsto> t\<^sub>1) \<turnstile>\<^sub>n e' : t'" by simp
+  with 3 X have "\<Gamma>(?z \<mapsto> t\<^sub>1) \<turnstile>\<^sub>n subst\<^sub>s x e' (subst_var\<^sub>s y ?z e) : t\<^sub>2" by fastforce
+  with T show ?case by (simp add: Let_def)
+qed fastforce+
+
+theorem preservationn: "e \<Down> v \<Longrightarrow> \<Gamma> \<turnstile>\<^sub>n e : t \<Longrightarrow> \<Gamma> \<turnstile>\<^sub>n v : t"
+  by (induction e v arbitrary: t rule: eval\<^sub>s.induct) fastforce+
+
+end
